Take advantage of separate accept/reject in ConfigMeaning

TwoWayAutomata/Kozen/Correctness.lean
@@ -18,22 +18,31 @@ namespace TwoDFA
 
 structure ConfigMeaning (n : Nat) (α σ : Type*) : Type _ where
   --- Meaning of being in the given state at the left end marker
-  atLeft : State σ → Vector α n → Prop
+  atLeft : σ → Vector α n → Prop
   --- Meaning of being in the given state at the given position in the input after the left endmarker
-  inWord : State σ → SplitPredicate n α 
+  inWord : σ → SplitPredicate n α 
+  --- Meaning of being in the accept state
+  accept : Vector α n → Prop
+  --- Meaning of being in the reject state
+  reject : Vector α n → Prop
 
 namespace ConfigMeaning
 
+@[reducible]
 def apply (cm : ConfigMeaning n α σ) (w : Word α n) (cfg : Config σ n) : Prop :=
-  if hcfg : cfg.idx = 0
-    then
-      cm.atLeft cfg.state w.val
-    else
-      cm.inWord cfg.state |>.apply w cfg.idx hcfg
+  match cfg with
+  | ⟨.accept, _⟩ => cm.accept w.val
+  | ⟨.reject, _⟩ => cm.reject w.val
+  | ⟨.other q, i⟩ =>
+    if hcfg : i = 0
+      then
+        cm.atLeft q w.val
+      else
+        cm.inWord q |>.apply w i hcfg
 
 structure Inductive (m : TwoDFA α σ) (cm : ConfigMeaning n α σ) : Prop where
   base : ∀ w, cm.apply w m.init
-  ind : ∀ w, ∀ cfg : Config σ n, cm.apply w cfg → cm.apply w (m.stepConfig w cfg)
+  ind : ∀ w, ∀ (q : σ) (i : Fin _), cm.apply w ⟨q, i⟩ → cm.apply w (m.stepConfig w ⟨q, i⟩)
 
 theorem Inductive.apply_of_reachable {motive : ConfigMeaning n α σ} {m : TwoDFA α σ} (ind : motive.Inductive m)
   {w : Word α n} {cfg : Config σ n} (hgoes : m.reaches w cfg) :
@@ -41,9 +50,17 @@ theorem Inductive.apply_of_reachable {motive : ConfigMeaning n α σ} {m : TwoDF
   induction hgoes with
   | refl => exact ind.base w
   | @tail mid stp head tail head_ih =>
-    have hind := ind.ind w mid head_ih
-    have : m.stepConfig w mid = stp := by rwa [m.stepConfig_gives_nextConfig w mid stp]
-    rwa [this] at hind
+    match mid with
+    | ⟨.accept, _⟩ =>
+      have : stp = ⟨.accept, stp.idx⟩ := by ext <;> simp [tail.halt_preserve_state]
+      rw [this]; simpa -- uses head_ih
+    | ⟨.reject, _⟩ =>
+      have : stp = ⟨.reject, stp.idx⟩ := by ext <;> simp [tail.halt_preserve_state]
+      rw [this]; simpa -- uses head_ih
+    | ⟨.other q, i⟩ =>
+      have hind := ind.ind w q i head_ih
+      have : m.stepConfig w ⟨q, i⟩ = stp := by rwa [m.stepConfig_gives_nextConfig w ⟨q, i⟩ stp]
+      rwa [this] at hind
 
 end ConfigMeaning
 
@@ -63,16 +80,15 @@ theorem language_eq_of_inductive [Fintype σ] (m : TwoDFA α σ) (L : Language �
     apply reaches_accept_last_of_accepts
     assumption
   · intro
-    cases em (m.diverges w.toWord) with
-    | inl h =>
-      have : w ∉ L := hdiv h
+    by_cases h : m.diverges w.toWord
+    · have : w ∉ L := hdiv h
       contradiction
-    | inr h =>
-      rw [m.divergence_iff, ←or_iff_not_and_not] at h
-      cases h with
-      | inl => assumption -- _ : m.accepts w
-      | inr => -- _ : m.rejects w
-        suffices w ∉ L by contradiction
+    · rw [m.divergence_iff, ←or_iff_not_and_not] at h
+      cases h
+      -- m.accepts w
+      · assumption
+      -- m.rejects w
+      · suffices w ∉ L by contradiction
         apply hrej
         apply hind.apply_of_reachable
         apply reaches_reject_last_of_rejects
